Tweak new system call definitions and prove preservation

platform/Safety.v
@@ -64,6 +64,31 @@ Lemma get_memoryIn : forall m w,
   reflexivity.
 Qed.
 
+Require Import DepList.
+
+Fixpoint smem_put ls (sm : smem' ls) (w : W) (v : B) : smem' ls :=
+  match sm with
+    | HNil => HNil
+    | HCons w' _ v' sm' =>
+      HCons (if H.addr_dec w w' then Some v else v') (smem_put _ sm' w v)
+  end.
+
+Fixpoint smem_clear ls (sm : smem' ls) (w : W) : smem' ls :=
+  match sm with
+    | HNil => HNil
+    | HCons w' _ v sm' =>
+      HCons (if H.addr_dec w w' then None else v) (smem_clear _ sm' w)
+  end.
+
+Fixpoint smem_graft (sm sm' : smem) (p : W) (len : nat) : smem :=
+  match len with
+    | O => sm
+    | S len' =>
+      match smem_get p sm' with
+        | None => sm
+        | Some v => smem_put _ (smem_graft sm sm' (p ^+ $1) len') p v
+      end
+  end.
 
 Section OpSem.
   Variable m : module.
@@ -263,8 +288,6 @@ Section OpSem.
     congruence.
   Qed.
 
-  Hint Unfold onlyChange.
-
   Lemma prove_ReadWord : forall stn m (p : W) v st,
     evalInstrs stn st (Assign Rv (LvMem p) :: nil) <> None
     -> (forall st', evalInstrs stn st (Assign Rv (LvMem p) :: nil) = Some st'
@@ -301,6 +324,760 @@ Section OpSem.
     apply specs_hit in H; post; eauto.
     apply specs'_hit in H0; post; eauto.
   Qed.
+
+  Lemma smem_get'_emp : forall p ls,
+    smem_get' ls p (smem_emp' ls) = None.
+    induction ls; simpl; intuition.
+    destruct (H.addr_dec a p); auto.
+  Qed.
+
+  Lemma smem_get_emp : forall p,
+    smem_get p smem_emp = None.
+    intros; apply smem_get'_emp.
+  Qed.
+
+  Lemma must_be' : forall p ls m1 m2,
+    smem_get' ls p m1 = None
+    -> smem_get' ls p m2 = None
+    -> smem_get' ls p (join' ls m1 m2) = None.
+    clear; induction ls; simpl; intuition.
+    destruct (H.addr_dec a p); subst; intuition.
+    rewrite H; auto.
+  Qed.
+
+  Lemma must_be : forall m m1 m2 p,
+    split m m1 m2
+    -> smem_get p m <> None
+    -> smem_get p m1 = None
+    -> smem_get p m2 <> None.
+    destruct 1; intuition subst.
+    unfold smem_get, join in H1.
+    rewrite must_be' in H1; eauto.
+  Qed.
+
+  Lemma characterize_array8_fwd : forall specs stn bs base m m',
+    interp specs (array8 bs base stn m)
+    -> (forall p, (forall n, (n < length bs)%nat -> p <> base ^+ $(n))
+      -> smem_get p m' = smem_get p m)
+    -> (forall p, smem_get p m <> None ->
+      exists n, (n < length bs)%nat /\ p = base ^+ $(n)).
+    clear; induction bs; simpl; propxFo.
+
+    hnf in H3; subst.
+    rewrite smem_get_emp in H1; tauto.
+    destruct (weq p base); subst.
+    exists 0; intuition.
+    unfold H.addr in *; W_eq.
+
+    assert (smem_get p x0 <> None).
+    eapply must_be; eauto.
+    case_eq (smem_get p x0); intros; try congruence.
+    clear H.
+    edestruct IHbs; eauto.
+    instantiate (1 := p); congruence.
+    intuition subst.
+    exists (S x1); intuition.
+    change ($(S x1)) with (natToW (S x1)).
+    rewrite (natToW_S x1).
+    unfold natToW.
+    unfold H.addr in *.
+    W_eq.
+  Qed.
+
+  Lemma split_None : forall p m m1 m2,
+    smem_get p m = None
+    -> split m m1 m2
+    -> smem_get p m2 = None.
+    intros; case_eq (smem_get p m2); intros; auto.
+    eapply split_smem_get in H0; eauto.
+    congruence.
+  Qed.
+
+  Lemma split'_None' : forall p ls m1 m2,
+    smem_get' ls p m1 = None
+    -> smem_get' ls p m2 = smem_get' ls p (join' ls m1 m2).
+    induction ls; simpl; intuition.
+    destruct (H.addr_dec a p); subst; intuition.
+    rewrite H; auto.
+  Qed.
+
+  Lemma split_None' : forall p m m1 m2,
+    split m m1 m2
+    -> smem_get p m1 = None
+    -> smem_get p m2 = smem_get p m.
+    destruct 1; subst; apply split'_None'.
+  Qed.
+
+  Lemma characterize_array8_bwd : forall specs stn bs base m,
+    interp specs (array8 bs base stn m)
+    -> (forall n, (n < length bs)%nat
+      -> smem_get (base ^+ $(n)) m <> None).
+    induction bs; simpl; propxFo.
+
+    intuition.
+
+    destruct n.
+    erewrite split_smem_get in H1.
+    discriminate.
+    eauto.
+    replace (base ^+ $0) with base by words.
+    eauto.
+
+    eapply IHbs.
+    eauto.
+    instantiate (1 := n); omega.
+    replace (base ^+ $1 ^+ $(n)) with (base ^+ $(S n))
+      by (rewrite natToW_S; unfold natToW; words).
+    eauto using split_None.
+  Qed.
+
+  Lemma semp_eta' : forall ls, NoDup ls
+    -> forall m,
+      (forall p, In p ls -> smem_get' ls p m = None)
+      -> m = smem_emp' ls.
+    clear; induction 1; simpl; intuition.
+    rewrite (hlist_nil_only _ m); auto.
+    rewrite (hlist_eta _ m); f_equal.
+    specialize (H1 x); destruct (H.addr_dec x x); tauto.
+    apply IHNoDup; intros.
+    specialize (H1 p); destruct (H.addr_dec x p); subst; eauto; tauto.
+  Qed.
+
+  Lemma semp_eta : forall m,
+    (forall p, smem_get p m = None)
+    -> semp m.
+    intros; apply semp_eta'; auto.
+    apply H.NoDup_all_addr.
+  Qed.
+
+  Lemma get_clear_ne' : forall a a' ls (sm : smem' ls),
+    a <> a'
+    -> smem_get' ls a (smem_clear _ sm a') = smem_get' ls a sm.
+    induction sm; simpl; intuition.
+    destruct (H.addr_dec x a); auto.
+    destruct (H.addr_dec a' x); congruence.
+  Qed.
+
+  Lemma get_clear_ne : forall a a' sm,
+    a <> a'
+    -> smem_get a (smem_clear _ sm a') = smem_get a sm.
+    intros; apply get_clear_ne'; auto.
+  Qed.
+
+  Lemma get_clear_eq' : forall a ls (sm : smem' ls),
+    smem_get' ls a (smem_clear _ sm a) = None.
+    induction sm; simpl; intuition.
+    destruct (H.addr_dec x a); auto.
+    destruct (H.addr_dec a x); congruence.
+  Qed.
+
+  Lemma get_clear_eq : forall a sm,
+    smem_get a (smem_clear _ sm a) = None.
+    intros; apply get_clear_eq'.
+  Qed.
+
+  Hint Rewrite get_clear_eq get_clear_ne
+    using solve [ assumption | W_neq ] : get.
+
+  Lemma get_put_eq' : forall a v ls (sm : smem' ls),
+    In a ls
+    -> smem_get' ls a (smem_put _ sm a v) = Some v.
+    induction sm; simpl; intuition.
+    subst.
+    destruct (H.addr_dec a a); intuition idtac.
+    destruct (H.addr_dec x a); intuition idtac.
+    subst.
+    destruct (H.addr_dec a a); intuition idtac.
+  Qed.
+
+  Lemma allWordsUpto_universal : forall width init w,
+    (wordToNat w < init)%nat
+    -> (init <= pow2 width)%nat
+    -> In w (allWordsUpto width init).
+    induction init; simpl; intuition.
+    destruct (weq w $(init)); subst; auto; right.
+    assert (wordToNat w <> init).
+    intro; apply n.
+    subst.
+    symmetry; apply natToWord_wordToNat.
+    auto.
+  Qed.
+
+  Lemma allWords_universal : forall sz w,
+    In w (allWords sz).
+    rewrite allWords_eq; intros; apply allWordsUpto_universal.
+    apply wordToNat_bound.
+    auto.
+  Qed.
+
+  Lemma get_put_eq : forall a v sm,
+    smem_get a (smem_put _ sm a v) = Some v.
+    intros; apply get_put_eq'.
+    apply allWords_universal.
+  Qed.
+
+  Lemma get_put_ne' : forall a a' v ls (sm : smem' ls),
+    a <> a'
+    -> smem_get' ls a (smem_put _ sm a' v) = smem_get' ls a sm.
+    induction sm; simpl; intuition.
+    destruct (H.addr_dec a' x); intuition idtac.
+    destruct (H.addr_dec x a); intuition idtac.
+    congruence.
+    destruct (H.addr_dec x a); intuition idtac.
+  Qed.
+
+  Lemma get_put_ne : forall a a' v sm,
+    a <> a'
+    -> smem_get a (smem_put _ sm a' v) = smem_get a sm.
+    intros; apply get_put_ne'; auto.
+  Qed.
+
+  Hint Rewrite smem_get_emp get_put_eq get_put_ne
+    using solve [ assumption | W_neq ] : get.
+
+  Lemma join_None' : forall a ls sm1 sm2,
+    smem_get' ls a sm1 = None
+    -> smem_get' ls a (join' ls sm1 sm2) = smem_get' ls a sm2.
+    induction sm1; simpl; intuition.
+    destruct (H.addr_dec x a); subst; auto.
+  Qed.
+
+  Lemma join_None : forall a sm1 sm2,
+    smem_get a sm1 = None
+    -> smem_get a (join sm1 sm2) = smem_get a sm2.
+    intros; apply join_None'; auto.
+  Qed.
+
+  Lemma join_Some' : forall a v ls sm1 sm2,
+    smem_get' ls a sm1 = Some v
+    -> smem_get' ls a (join' ls sm1 sm2) = Some v.
+    induction sm1; simpl; intuition.
+    destruct (H.addr_dec x a); subst; auto.
+  Qed.
+
+  Lemma join_Some : forall a v sm1 sm2,
+    smem_get a sm1 = Some v
+    -> smem_get a (join sm1 sm2) = Some v.
+    intros; apply join_Some'; auto.
+  Qed.
+
+  Lemma disjoint_get' : forall ls sm1 sm2,
+    NoDup ls
+    -> List.Forall (fun w => smem_get' ls w sm1 <> None -> smem_get' ls w sm2 <> None -> False) ls
+    -> disjoint' ls sm1 sm2.
+    induction sm1; simpl; intuition; rewrite (hlist_eta _ sm2) in *; simpl in *.
+    inversion H; clear H; subst.
+    inversion H0; clear H0; subst.
+    destruct (H.addr_dec x x); try tauto.
+    destruct b; auto.
+    destruct (hlist_hd sm2); auto.
+    intuition discriminate.
+    inversion H; clear H; subst.
+    inversion H0; clear H0; subst.
+    apply IHsm1; intros; auto.
+    eapply Forall_weaken'; eauto.
+    simpl; intros.
+    destruct (H.addr_dec x x0); subst; tauto.
+  Qed.
+
+  Lemma disjoint_get : forall sm1 sm2,
+    (forall w, smem_get w sm1 <> None -> smem_get w sm2 <> None -> False)
+    -> disjoint sm1 sm2.
+    intros; apply disjoint_get'.
+    apply BedrockHeap.NoDup_all_addr.
+    apply Forall_forall; intros.
+    eauto.
+  Qed.
+
+  Lemma disjoint_get_fwd' : forall ls sm1 sm2,
+    disjoint' ls sm1 sm2
+    -> NoDup ls
+    -> List.Forall (fun w => smem_get' ls w sm1 <> None -> smem_get' ls w sm2 <> None -> False) ls.
+    induction sm1; simpl; intuition; rewrite (hlist_eta _ sm2) in *; simpl in *;
+      subst; constructor; simpl.
+    destruct (H.addr_dec x x); tauto.
+    inversion H0; clear H0; subst.
+    eapply Forall_weaken'; try apply IHsm1.
+    eauto.
+    auto.
+    simpl; intros.
+    destruct (H.addr_dec x x0); subst; tauto.
+    destruct (H.addr_dec x x); tauto.
+    inversion H0; clear H0; subst.
+    eapply Forall_weaken'; try apply IHsm1.
+    eauto.
+    auto.
+    simpl; intros.
+    destruct (H.addr_dec x x0); subst; tauto.
+  Qed.
+
+  Lemma disjoint_get_fwd : forall sm1 sm2,
+    disjoint sm1 sm2
+    -> (forall w, smem_get w sm1 <> None -> smem_get w sm2 <> None -> False).
+    intros; eapply disjoint_get_fwd' in H; try apply BedrockHeap.NoDup_all_addr.
+    assert (In w H.all_addr) by apply allWords_universal.
+    generalize (proj1 (Forall_forall _ _) H _ H2); tauto.
+  Qed.
+
+  Lemma smem_eta : forall ls (sm sm' : smem' ls),
+    NoDup ls
+    -> List.Forall (fun w => smem_get' ls w sm = smem_get' ls w sm') ls
+    -> sm = sm'.
+    induction sm; simpl; intuition.
+    rewrite hlist_nil; auto.
+    inversion H0; clear H0; subst.
+    inversion H; clear H; subst.
+    destruct (H.addr_dec x x); intuition idtac; subst.
+    rewrite (hlist_eta _ sm'); f_equal.
+    apply IHsm; auto.
+    eapply Forall_weaken'; eauto.
+    simpl; intros.
+    destruct (H.addr_dec x x0); subst; tauto.
+  Qed.
+
+  Lemma split_put_clear : forall sm sm1 sm2 a v,
+    split sm sm1 sm2
+    -> smem_get a sm2 = Some v
+    -> split sm (smem_put _ sm1 a v) (smem_clear _ sm2 a).
+    unfold split; intuition subst.
+    apply disjoint_get; intros.
+    destruct (weq w a); subst.
+    autorewrite with get in *; tauto.
+    autorewrite with get in *.
+    eapply disjoint_get_fwd in H1; eassumption.
+
+    apply smem_eta; try apply BedrockHeap.NoDup_all_addr.
+    apply Forall_forall; intros.
+    destruct (weq x a); subst.
+    rewrite join_None.
+    erewrite join_Some.
+    eauto.
+    autorewrite with get; reflexivity.
+    case_eq (smem_get a sm1); auto; intros.
+    eapply disjoint_get_fwd in H1; try eassumption.
+    tauto.
+    instantiate (1 := a); congruence.
+    congruence.
+    
+    case_eq (smem_get x sm1); intros.
+    erewrite join_Some.
+    erewrite join_Some.
+    2: autorewrite with get; eassumption.
+    2: eassumption.
+    reflexivity.
+
+    rewrite join_None.
+    rewrite join_None.
+    autorewrite with get; reflexivity.
+    autorewrite with get; assumption.
+    assumption.
+  Qed.
+
+  Lemma recharacterize_array8 : forall specs stn sz base m,
+    (forall n, (0 < n < sz)%nat
+      -> base ^+ $(n) <> base)
+    -> (forall n, (n < sz)%nat
+      -> smem_get (base ^+ $(n)) m <> None)
+    -> (forall p, smem_get p m <> None ->
+      exists n, (n < sz)%nat /\ p = base ^+ $(n))
+    -> exists bs, length bs = sz /\ interp specs (array8 bs base stn m).
+    clear; induction sz; simpl; intuition.
+
+    exists nil; simpl; propxFo.
+    apply semp_eta.
+    intros.
+    specialize (H1 p).
+    destruct (smem_get p m); auto.
+    destruct H1.
+    congruence.
+    intuition.
+
+    generalize (H0 0); replace (base ^+ $0) with base by words;
+      case_eq (smem_get base m); intros; try solve [ elimtype False; eauto ].
+    clear H3.
+    edestruct IHsz.
+    instantiate (1 := base ^+ $1).
+    intros.
+    replace (base ^+ $ (1) ^+ $ (n)) with (base ^+ natToW (S n)) in *
+      by (rewrite natToW_S; unfold natToW; W_eq).
+    intros.
+    eapply H.
+    instantiate (1 := n); auto.
+    apply (f_equal (fun x => x ^- $1)) in H4.
+    rewrite natToW_S in H4.
+    unfold natToW in H4.
+    replace (base ^+ ($1 ^+ $(n)) ^- $1) with (base ^+ $(n)) in H4 by W_eq.
+    replace (base ^+ $1 ^- $1) with base in H4 by W_eq.
+    auto.
+
+    instantiate (1 := smem_clear _ m base).
+    intros.
+    replace (base ^+ $ (1) ^+ $ (n)) with (base ^+ natToW (S n)) in H4
+      by (rewrite natToW_S; unfold natToW; W_eq).
+    rewrite get_clear_ne in H4.
+    apply H0 with (S n).
+    auto.
+    auto.
+    intro.
+    eapply H.
+    2: eauto.
+    auto.
+
+    intros.
+    destruct (weq p base); subst.
+    rewrite get_clear_eq in H3; tauto.
+    rewrite get_clear_ne in H3; auto.
+    apply H1 in H3.
+    propxFo; subst.
+    destruct x.
+    elimtype False; apply n.
+    words.
+    exists x; intuition.
+    rewrite natToW_S.
+    unfold natToW.
+    unfold H.addr in *.
+    W_eq.
+
+    intuition subst; simpl; exists (b :: x); propxFo.
+    exists (smem_put _ smem_emp base b).
+    exists (smem_clear _ m base).
+    descend.
+    apply split_put_clear.
+    apply split_a_semp_a.
+    auto.
+    apply get_put_eq.
+    rewrite get_put_ne; auto.
+    autorewrite with get; auto.
+  Qed.
+
+  Lemma disjoint_eta' : forall ls, NoDup ls
+    -> forall m1 m2,
+      (forall p v1 v2, In p ls
+        -> smem_get' ls p m1 = Some v1
+        -> smem_get' ls p m2 = Some v2
+        -> False)
+      -> disjoint' ls m1 m2.
+    induction 1; simpl; intuition auto 1.
+    specialize (H1 x); destruct (H.addr_dec x x); try tauto.
+    destruct (hlist_hd m1); auto; destruct (hlist_hd m2); auto.
+    elimtype False; eauto.
+
+    apply IHNoDup; intros.
+    specialize (H1 p).
+    destruct (H.addr_dec x p); try congruence.
+    eauto.
+  Qed.
+
+  Lemma disjoint_eta : forall m1 m2,
+    (forall p v1 v2, smem_get p m1 = Some v1
+      -> smem_get p m2 = Some v2
+      -> False)
+    -> disjoint m1 m2.
+    intros; apply disjoint_eta'.
+    apply H.NoDup_all_addr.
+    eauto.
+  Qed.
+
+  Lemma get_graft : forall p0 v sz m m' p,
+    smem_get p0 (smem_graft m m' p sz) = Some v
+    -> smem_get p0 m = Some v \/ (exists n, p0 = p ^+ $(n)
+      /\ (n < sz)%nat
+      /\ smem_get p0 m' = Some v).
+    clear; induction sz; simpl; intuition auto 1.
+    case_eq (smem_get p m'); intros;
+      match goal with
+        | [ H : _ = _ |- _ ] => rewrite H in *; try congruence; eauto
+      end.
+    destruct (weq p0 p); subst.
+    rewrite get_put_eq in *.
+    right; exists 0; intuition.
+    unfold H.addr in *; W_eq.
+    rewrite get_put_ne in *; eauto.
+    destruct (IHsz _ _ _ H) as [ | [ ? [ ] ] ]; subst; intuition eauto.
+    right; exists (S x); intuition.
+    unfold H.addr in *.
+    change ($ (S x)) with (natToW (S x)).
+    rewrite (natToW_S x).
+    unfold natToW in *; words.
+  Qed.
+
+  Lemma disjoint_not_both' : forall p v ls m1 m2,
+    disjoint' ls m1 m2
+    -> smem_get' ls p m2 = Some v
+    -> smem_get' ls p m1 = None.
+    clear; induction ls; simpl; intuition.
+
+    destruct (H.addr_dec a p); eauto.
+
+    destruct (H.addr_dec a p); eauto; congruence.
+  Qed.
+
+  Lemma disjoint_not_both : forall m1 m2 p v,
+    disjoint m1 m2
+    -> smem_get p m2 = Some v
+    -> smem_get p m1 = None.
+    intros; eapply disjoint_not_both'; eauto.
+  Qed.
+
+  Lemma smem_canon' : forall ls, NoDup ls
+    -> forall m1 m2,
+      (forall p, In p ls -> smem_get' ls p m1 = smem_get' ls p m2)
+      -> m1 = m2.
+    clear; induction 1; simpl; intuition.
+    rewrite (hlist_nil_only _ m1); rewrite (hlist_nil_only _ m2); auto.
+    rewrite (hlist_eta _ m1); rewrite (hlist_eta _ m2).
+    f_equal.
+    specialize (H1 x); destruct (H.addr_dec x x); tauto.
+    apply IHNoDup; intros.
+    specialize (H1 p).
+    destruct (H.addr_dec x p).
+    congruence.
+    auto.
+  Qed.
+
+  Lemma smem_canon : forall m1 m2,
+    (forall p, smem_get p m1 = smem_get p m2)
+    -> m1 = m2.
+    intros; apply smem_canon'.
+    apply H.NoDup_all_addr.
+    auto.
+  Qed.
+
+  Fixpoint smem_minus' ls : smem' ls -> smem' ls -> smem' ls :=
+    match ls with
+      | nil => fun sm _ => sm
+      | a :: ls' => fun sm sm' =>
+        HCons match hlist_hd sm' with
+                | Some _ => None
+                | _ => hlist_hd sm
+              end (smem_minus' _ (hlist_tl sm) (hlist_tl sm'))
+    end.
+
+  Definition smem_minus (sm sm' : smem) := smem_minus' _ sm sm'.
+
+  Lemma disjoint_minus' : forall ls, NoDup ls
+    -> forall m m',
+      (forall p v, In p ls
+        -> smem_get' ls p m' = Some v -> smem_get' ls p m = Some v)
+      -> disjoint' ls (smem_minus' _ m m') m'.
+    clear; induction 1; simpl; intuition.
+    specialize (H1 x).
+    destruct (H.addr_dec x x); try tauto.
+    destruct (hlist_hd m'); eauto.
+    apply IHNoDup; intros.
+    specialize (H1 p); destruct (H.addr_dec x p); try congruence.
+    eauto.
+  Qed.
+
+  Lemma disjoint_minus : forall m m',
+    (forall p v, smem_get p m' = Some v -> smem_get p m = Some v)
+    -> disjoint (smem_minus' _ m m') m'.
+    intros; apply disjoint_minus'; auto.
+    apply H.NoDup_all_addr.
+  Qed.
+
+  Lemma join_minus' : forall ls, NoDup ls
+    -> forall m m',
+      (forall p v, In p ls
+        -> smem_get' ls p m' = Some v -> smem_get' ls p m = Some v)
+      -> m = join' ls (smem_minus' _ m m') m'.
+    clear; induction 1; simpl; intuition.
+    rewrite (hlist_nil_only _ m); auto.
+    rewrite (hlist_eta _ m); simpl; f_equal.
+    specialize (H1 x); destruct (H.addr_dec x x); try tauto.
+    destruct (hlist_hd m'); eauto.
+    destruct (hlist_hd m); auto.
+    
+    apply IHNoDup; intros.
+    specialize (H1 p); destruct (H.addr_dec x p); subst.
+    tauto.
+    eauto.
+  Qed.
+
+  Lemma join_minus : forall m m',
+    (forall p v, smem_get p m' = Some v -> smem_get p m = Some v)
+    -> m = join (smem_minus' _ m m') m'.
+    intros; apply join_minus'; auto.
+    apply H.NoDup_all_addr.
+  Qed.
+
+  Lemma split_minus : forall m m',
+    (forall p v, smem_get p m' = Some v -> smem_get p m = Some v)
+    -> split m (smem_minus m m') m'.
+    unfold split; intuition subst; auto using disjoint_minus, join_minus.
+  Qed.
+
+  Lemma no_overlap' : forall p v1 v2 ls m1 m2,
+    disjoint' ls m1 m2
+    -> In p ls
+    -> smem_get' ls p m1 = Some v1
+    -> smem_get' ls p m2 = Some v2
+    -> False.
+    induction ls; simpl; intuition subst.
+    destruct (H.addr_dec p p); try tauto; congruence.
+    destruct (H.addr_dec p p); try tauto; congruence.
+    destruct (H.addr_dec a p); eauto; congruence.
+    destruct (H.addr_dec a p); eauto; congruence.
+  Qed.
+
+  Lemma no_overlap : forall m1 m2 p v1 v2,
+    disjoint m1 m2
+    -> smem_get p m1 = Some v1
+    -> smem_get p m2 = Some v2
+    -> False.
+    intros; eapply no_overlap'; eauto.
+    apply allWords_universal.
+  Qed.
+
+  Lemma not_zero : forall sz n,
+    (0 < n < pow2 sz)%nat
+    -> natToWord sz n <> wzero sz.
+    intros; intro.
+    apply (f_equal (@wordToNat _)) in H0.
+    rewrite wordToNat_natToWord_idempotent in H0.
+    subst.
+    rewrite roundTrip_0 in H.
+    omega.
+    pre_nomega.
+    rewrite Npow2_nat.
+    auto.
+  Qed.
+
+  Lemma tickle_bytes : forall specs p sz P stn st st',
+    interp specs (![ p =?>8 sz * P] (stn, st))
+    -> onlyChange p sz (Mem st) (Mem st')
+    -> interp specs (![ p =?>8 sz * P] (stn, st')).
+    clear; rewrite sepFormula_eq.
+    intros.
+    apply simplify_fwd in H; simpl in *.
+    repeat match goal with
+             | [ H : Logic.ex _ |- _ ] => destruct H
+             | [ H : _ /\ _ |- _ ] => destruct H
+           end.
+    apply simplify_bwd in H3.
+    hnf in H5; subst.
+    apply split_comm in H1; apply split_semp in H1; try reflexivity; subst.
+
+    edestruct recharacterize_array8.
+
+    instantiate (1 := p).
+    instantiate (1 := length x1).
+    intros.
+    apply word_neq.
+    replace (p ^+ $(n) ^- p) with (natToW n).
+    apply not_zero.
+    eapply array8_bound in H3.
+    generalize dependent 32.
+    intros.
+    omega.
+    unfold H.addr, natToW in *; W_eq.
+
+    instantiate (1 := smem_minus (memoryIn (Mem st')) x0).
+    intros.
+    eapply characterize_array8_bwd in H3; eauto.
+
+    Lemma get_minus_out' : forall p ls m1 m2,
+      smem_get' ls p m2 = None
+      -> smem_get' ls p (smem_minus' _ m1 m2) = smem_get' ls p m1.
+      clear; induction ls; simpl; intuition.
+      destruct (H.addr_dec a p); intuition.
+      rewrite H; auto.
+    Qed.
+
+    Lemma get_minus_out : forall p m1 m2,
+      smem_get p m2 = None
+      -> smem_get p (smem_minus m1 m2) = smem_get p m1.
+      intros; apply get_minus_out'; auto.
+    Qed.
+
+    Lemma get_minus_in' : forall p ls m1 m2,
+      smem_get' ls p m2 <> None
+      -> smem_get' ls p (smem_minus' _ m1 m2) = None.
+      clear; induction ls; simpl; intuition.
+      destruct (H.addr_dec a p); intuition.
+      destruct (hlist_hd m2); tauto.
+    Qed.
+
+    Lemma get_minus_in : forall p m1 m2,
+      smem_get p m2 <> None
+      -> smem_get p (smem_minus m1 m2) = None.
+      intros; apply get_minus_in'; auto.
+    Qed.
+
+    rewrite get_minus_out.
+    case_eq (smem_get (p ^+ $(n)) x2); intros; try congruence.
+    eapply unsplit_smem_get in H4; eauto.
+    repeat rewrite get_memoryIn in *.
+    destruct H0.
+    specialize (SameMapped (p ^+ $(n))).
+    intuition.
+
+    case_eq (smem_get (p ^+ $ (n)) x2); intros; try congruence.
+    case_eq (smem_get (p ^+ $ (n)) x0); intros; try congruence.
+    destruct H.
+    elimtype False; eapply no_overlap; eauto.
+
+    intros.
+    destruct H0.
+    eapply characterize_array8_fwd; eauto.
+    case_eq (smem_get p0 x0); intros.
+    rewrite get_minus_in in H1; congruence.
+    rewrite get_minus_out in H1 by congruence.
+    assert (smem_get p0 (memoryIn (Mem st)) <> None).
+    repeat rewrite get_memoryIn in *.
+    specialize (SameMapped p0); intuition.
+    eapply must_be; eauto; apply split_comm; auto.
+
+    intuition.
+    propxFo.
+    descend.
+    apply split_minus; intros.
+    assert (smem_get p0 (memoryIn (Mem st)) = Some v)
+      by (eapply split_smem_get; eauto).
+    repeat rewrite get_memoryIn in *.
+    destruct H0.
+    rewrite Elsewhere; auto.
+    intros.
+    destruct (weq p0 (p ^+ $(n))); subst; auto.
+    eapply characterize_array8_bwd in H3; eauto.
+    case_eq (smem_get (p ^+ $(n)) x2); intros; try congruence.
+    destruct H; intro; eauto using no_overlap.
+
+    apply split_comm; apply split_a_semp_a.
+
+    eauto.
+    eauto.
+    reflexivity.
+    auto.
+  Qed.
+
+  Ltac eqer := repeat (match goal with
+                         | [ H : _ = _ |- _ ] => rewrite H in *
+                         | [ H : Some _ = Some _ |- _ ] =>
+                           injection H; clear H; intros
+                         | [ H : Logic.ex _ |- _ ] => destruct H; try clear H
+                         | [ H : _ /\ _ |- _ ] => destruct H; try clear H
+                       end; subst).
+
+  Lemma onlyChange_refl : forall p len m,
+    onlyChange p len m m.
+    constructor; intuition.
+  Qed.
+
+  Hint Immediate onlyChange_refl.
+
+  Ltac prove_ReadWord :=
+    eapply prove_ReadWord; hnf; intros; cbv beta in *;
+      try rewrite evalInstrs_slot in *;
+        match goal with
+          | [ st : (W * state)%type |- _ ] => destruct st; simpl in *
+          | [ st : state' |- _ ] => destruct st; simpl in *
+        end;
+        generalize dependent (specs m stn); intros;
+          repeat match goal with
+                   | [ H : interp _ _ |- _ ] => generalize dependent H
+                   | [ H : context[evalInstrs] |- _ ] => generalize dependent H
+                 end; clear; intros; evaluate auto_ext; auto.
 
   Lemma progress : forall st, goodState st
     -> exists st', sys_step stn prog st st'.
@@ -345,12 +1122,7 @@ Section OpSem.
               | exists (st#Rp, snd st); eapply Read; eauto;
                 match goal with
                   | [ H : interp _ _ |- ReadWord ?stn (Mem (snd ?st)) _ = Some _ ] =>
-                    generalize H; clear; intros;
-                      apply prove_ReadWord with (snd st); hnf; intros; cbv beta in *;
-                        try rewrite evalInstrs_slot in *;
-                          generalize dependent (snd st);
-                            generalize dependent (specs m stn); intros;
-                              evaluate auto_ext; auto
+                    generalize H; clear; intros; prove_ReadWord
                 end ]
         end.
 
@@ -361,13 +1133,7 @@ Section OpSem.
             clear Hb; post;
               specialize (agree _ _ _ H); destruct agree as [ ? [ ] ]
     end;
-    repeat (match goal with
-              | [ H : _ = _ |- _ ] => rewrite H in *
-              | [ H : Some _ = Some _ |- _ ] =>
-                injection H; clear H; intros
-              | [ H : Logic.ex _ |- _ ] => destruct H; try clear H
-              | [ H : _ /\ _ |- _ ] => destruct H; try clear H
-            end; subst);
+    eqer;
     match goal with
       | [ H : specs _ _ _ = Some _ |- _ ] =>
         apply specs_hit in H; post; eauto
@@ -378,96 +1144,86 @@ Section OpSem.
       end.
   Qed.
 
+  Lemma goOnIn : forall P Q R,
+    Q * (P * R) ===> P * Q * R.
+    clear; sepLemma.
+  Qed.
+
   Lemma preservation : forall st, goodState st
     -> forall st', sys_step stn prog st st'
       -> goodState st'.
-    unfold goodState; destruct 2; post.
+    unfold goodState; destruct 2; post;
+      try match goal with
+            | [ x : label, H : _ |- _ ] =>
+              solve [ destruct x; specialize (impSys' _ _ H);
+                intro Hi; hnf in Hi; unfold labelSys' in Hi; simpl in Hi;
+                  intuition subst;
+                    match goal with
+                      | [ H : _ |- _ ] => apply omitImp in H;
+                        match goal with
+                          | [ H' : prog _ = None |- _ ] => 
+                            unfold step in *; rewrite H' in *; discriminate
+                        end
+                    end ]
 
-    specialize (impSys' _ _ H2); intro Hi; hnf in Hi; intuition subst.
-    apply omitImp in H1.
-    unfold step in H0.
-    rewrite H1 in H0; discriminate.
-    apply omitImp in H1.
-    unfold step in H0.
-    rewrite H1 in H0; discriminate.
+            | [ H : LabelMap.MapsTo _ _ (Blocks _), H' : interp _ _ |- _ ] =>
+              solve [ specialize (BlocksOk ok H); intro Hb; hnf in Hb;
+                apply Hb in H'; [ | eapply specsOk; eauto ];
+                  clear Hb; post;
+                    specialize (agree _ _ _ H); destruct agree as [ ? [ ] ];
+                      unfold step in *; eqer;
+                        apply specs_hit in H4; destruct H4; intuition idtac;
+                          try match goal with
+                                | [ H : Logic.ex _ |- _ ] => destruct H
+                              end; eauto 10 ]
 
-    specialize (BlocksOk ok H2); intro Hb; hnf in Hb.
-    apply Hb in H; [ | eapply specsOk; eauto ].
-    clear Hb; post.
-    specialize (agree _ _ _ H2); destruct agree as [ ? [ ] ].
-    rewrite H1 in H; injection H; clear H; intros; subst.
-    unfold step in H0.
-    rewrite H6 in H0.
-    rewrite H0 in H3; injection H3; clear H3; intros; subst.
-    apply specs_hit in H4; destruct H4; intuition idtac.
-    eauto 10.
-    destruct H; eauto 10.
-
-    specialize (impSys' _ _ H3); intro Hi; hnf in Hi; intuition subst.
-    eapply (inj _ _ _ H0) in H2; discriminate. 
-    post.
-    apply specs_hit in H5; destruct H5; intuition idtac.
-    descend.
-    eauto.
-    2: eauto.
-    descend; step auto_ext.
-    descend; eauto.
-    descend.
-    eauto.
-    2: eauto.
-    descend; step auto_ext.
-    descend; eauto.
-
-    apply (inj _ _ _ H0) in H2.
-    subst.
-    specialize (omitImp _ _ H0).
-    apply agree in H3.
-    post.
-    congruence.
-
-    specialize (impSys' _ _ H3); intro Hi; hnf in Hi; intuition subst.
-    eapply (inj _ _ _ H0) in H2; discriminate. 
-    post.
-    apply specs_hit in H5; destruct H5; intuition idtac.
-    descend.
-    eauto.
-    2: eauto.
-    descend; step auto_ext.
-    descend; eauto.
-    descend.
-    eauto.
-    2: eauto.
-    descend; step auto_ext.
-    descend; eauto.
-
-    apply (inj _ _ _ H0) in H2.
-    subst.
-    specialize (omitImp _ _ H0).
-    apply agree in H3.
-    post.
-    congruence.
-
-    specialize (impSys' _ _ H3); intro Hi; hnf in Hi; intuition subst.
-    eapply (inj _ _ _ H0) in H2; discriminate. 
-    post.
-    apply specs_hit in H5; destruct H5; intuition idtac.
-    descend.
-    eauto.
-    2: eauto.
-    descend; step auto_ext.
-    descend; eauto.
-    descend.
-    eauto.
-    2: eauto.
-    descend; step auto_ext.
-    descend; eauto.
-
-    apply (inj _ _ _ H0) in H2.
-    subst.
-    specialize (omitImp _ _ H0).
-    apply agree in H3.
-    post.
-    congruence.
+            | [ H1 : _, H2 : _ |- _ ] =>
+              solve [ apply (inj _ _ _ H1) in H2; subst;
+                specialize (omitImp _ _ H1);
+                  match goal with
+                    | [ H : _ |- _ ] => apply agree in H; post; congruence
+                  end ]
+          end;
+      match goal with
+        | [ x : label, H5 : LabelMap.MapsTo _ _ (Imports _) |- _ ] =>
+          destruct x; specialize (impSys' _ _ H5);
+            intro Hi; hnf in Hi; unfold labelSys' in Hi; simpl in Hi;
+              intuition subst;
+                match goal with
+                  | [ H : (_, _) = (_, _) |- _ ] =>
+                    injection H; clear H; intros; subst
+                end; eauto; post;
+                try match goal with
+                      | [ H1 : _, H2 : _ |- _ ] =>
+                        solve [ apply (inj _ _ _ H1) in H2;
+                          cbv beta in H2; congruence ]
+                    end; post;
+                match goal with
+                  | [ H : _ = _ |- _ ] => apply specs_hit in H; destruct H; intuition idtac
+                end;
+                match goal with
+                  | [ st' : state |- _ ] => destruct st'; simpl in *; subst
+                end; descend; eauto;
+                match goal with
+                  | [ H : forall x : ST.settings * state, _ |- _ ] =>
+                    apply (Imply_sound (H _)); propxFo; descend;
+                      try (apply ILTacCommon.ignore_regs; eassumption)
+                end
+      end;
+      match goal with
+        | [ H : interp (specs _ ?stn) (![?P] (_, snd ?st))%PropX |- _ ] =>
+          match P with
+            | context[locals _ ?V _ _] =>
+              eapply ILTacCommon.interp_interp_himp in H; [ | apply comeOnOut ];
+                eapply ILTacCommon.interp_interp_himp; [ | apply goOnIn ];
+                  eapply tickle_bytes; eauto;
+                    assert (ReadWord stn (IL.Mem (snd st)) (st#Sp ^+ $8)
+                      = Some (sel V "buffer")) by prove_ReadWord;
+                    assert (ReadWord stn (IL.Mem (snd st)) (st#Sp ^+ $12)
+                      = Some (sel V "size")) by prove_ReadWord;
+                    cbv beta in *; simpl; congruence
+          end
+      end.
   Qed.
 
   Lemma safety' : forall st, goodState st
